record...
Signed-off-by: Shaobo He <shaobohe@amazon.com>

cedar-lean/Cedar/Thm/Validation/WellTyped/Definition.lean
@@ -282,9 +282,9 @@ inductive TypedExpr.WellTyped (env : Environment) : TypedExpr → Prop
   (h₂ : ∀ x, x ∈ ls → x.typeOf = ty)
   (h₃ : ls != []) :
   WellTyped env (.set ls (.set ty))
-| record {m : List (Attr × TypedExpr)} {rty : Data.Map Attr QualifiedType}
+| record {rty : RecordType} {m : List (Attr × TypedExpr)}
   (h₁ : ∀ k v, (k,v) ∈ m → WellTyped env v)
-  (h₂ : List.Forall₂ (λ x y => x.fst = y.fst ∧ x.snd.typeOf = y.snd.getType) m rty.1) :
+  (h₂ : rty = Map.make (m.map (λ (a, ty) => (a, .required ty.typeOf)))) :
   WellTyped env (.record m (.record rty))
 | call {xfn : ExtFun} {args : List TypedExpr} {ty : CedarType}
   (h₁ : ∀ x, x ∈ args → WellTyped env x)
